wip

Foundation/Propositional/ConsistentTableau.lean
@@ -3,37 +3,46 @@ module
 public import Foundation.Propositional.Formula.Basic
 public import Foundation.Propositional.Entailment.Cl.Basic
 public import Foundation.Vorspiel.Set.Basic
+public import Foundation.Propositional.Entailment.Corsi
 
 @[expose] public section
 
 namespace LO.Propositional
 
-open Entailment FiniteContext
+open Entailment
 open Formula
 
 variable {α : Type*}
 variable {S} [Entailment S (Formula α)]
 variable {𝓢 : S}
 
-def Tableau (α : Type u) := Set (Formula α) × Set (Formula α)
+structure Tableau (α : Type u) where
+  Γ : Set (Formula α)
+  Δ : Set (Formula α)
 
 namespace Tableau
 
+instance : HasSubset (Tableau α) := ⟨λ t₁ t₂ => t₁.Γ ⊆ t₂.Γ ∧ t₁.Δ ⊆ t₂.Δ⟩
+
+def insert₁ (φ : Formula α) (t : Tableau α) : Tableau α := ⟨insert φ t.Γ, t.Δ⟩
+def insert₂ (φ : Formula α) (t : Tableau α) : Tableau α := ⟨t.Γ, insert φ t.Δ⟩
+
 variable {φ ψ: Formula α} {T U : FormulaSet α} {t u : Tableau α}
 
-abbrev Consistent (𝓢 : S) (t : Tableau α) := ∀ {Γ Δ : Finset (Formula α)}, (↑Γ ⊆ t.1) → (↑Δ ⊆ t.2) → 𝓢 ⊬ (Γ.conj) 🡒 (Δ.disj)
+@[grind]
+def Consistent (𝓢 : S) (t : Tableau α) := ∀ {Γ Δ : Finset (Formula α)}, (↑Γ ⊆ t.Γ) → (↑Δ ⊆ t.Δ) → 𝓢 ⊬ (Γ.conj) 🡒 (Δ.disj)
 
 abbrev Inconsistent (𝓢 : S) (t : Tableau α) := ¬Consistent 𝓢 t
+lemma iff_inconsistent : Inconsistent 𝓢 t ↔ ∃ Γ Δ : Finset (Formula α), (↑Γ ⊆ t.Γ) ∧ (↑Δ ⊆ t.Δ) ∧ 𝓢 ⊢ (Γ.conj) 🡒 (Δ.disj) := by grind;
 
-instance : HasSubset (Tableau α) := ⟨λ t₁ t₂ => t₁.1 ⊆ t₂.1 ∧ t₁.2 ⊆ t₂.2⟩
-@[simp] lemma subset_def {t₁ t₂ : Tableau α} : t₁ ⊆ t₂ ↔ t₁.1 ⊆ t₂.1 ∧ t₁.2 ⊆ t₂.2 := by rfl
+@[simp] lemma subset_def {t₁ t₂ : Tableau α} : t₁ ⊆ t₂ ↔ t₁.Γ ⊆ t₂.Γ ∧ t₁.Δ ⊆ t₂.Δ := by rfl
 
-@[simp] lemma equality_def {t₁ t₂ : Tableau α} : t₁ = t₂ ↔ t₁.1 = t₂.1 ∧ t₁.2 = t₂.2 := by
+@[simp] lemma equality_def {t₁ t₂ : Tableau α} : t₁ = t₂ ↔ t₁.Γ = t₂.Γ ∧ t₁.Δ = t₂.Δ := by
   constructor;
   . intro h; cases h; simp;
   . rintro ⟨h₁, h₂⟩; cases t₁; cases t₂; simp_all;
 
-lemma not_mem₂ (hCon : t.Consistent 𝓢) {Γ : Finset (Formula α)} (hΓ : ∀ φ ∈ Γ, φ ∈ t.1) (h : 𝓢 ⊢ Γ.conj 🡒 ψ) : ψ ∉ t.2 := by
+lemma not_mem₂ (hCon : t.Consistent 𝓢) {Γ : Finset (Formula α)} (hΓ : ∀ φ ∈ Γ, φ ∈ t.Γ) (h : 𝓢 ⊢ Γ.conj 🡒 ψ) : ψ ∉ t.Δ := by
   by_contra hC;
   have : 𝓢 ⊢ Γ.conj 🡒 (Finset.disj {ψ}) := by simpa;
   have : 𝓢 ⊬ Γ.conj 🡒 (Finset.disj {ψ}) := hCon (by aesop) (by aesop);
@@ -41,145 +50,113 @@ lemma not_mem₂ (hCon : t.Consistent 𝓢) {Γ : Finset (Formula α)} (hΓ : �
 
 section
 
-variable [Entailment.Int 𝓢]
+variable [Entailment.VF 𝓢]
+open Entailment.Corsi
 
-lemma disjoint_of_consistent (hCon : t.Consistent 𝓢) : Disjoint t.1 t.2 := by
+lemma disjoint_of_consistent (hCon : t.Consistent 𝓢) : Disjoint t.Γ t.Δ := by
   by_contra h;
   obtain ⟨T, hp₁, hp₂, hp⟩ := by simpa [Disjoint] using h;
   obtain ⟨φ, hp⟩ := Set.nonempty_def.mp $ Set.nonempty_iff_ne_empty.mpr hp;
-  have : 𝓢 ⊬ (Finset.conj {φ}) 🡒 (Finset.disj {φ}) := hCon
-    (by simp_all only [Finset.coe_singleton, Set.singleton_subset_iff]; apply hp₁; assumption)
-    (by simp_all only [Finset.coe_singleton, Set.singleton_subset_iff]; apply hp₂; assumption);
+  have : 𝓢 ⊬ (Finset.conj {φ}) 🡒 (Finset.disj {φ}) := hCon (by grind) (by grind);
   replace this : 𝓢 ⊬ φ 🡒 φ := by simpa using this;
-  have : 𝓢 ⊢ φ 🡒 φ := C!_id;
+  have : 𝓢 ⊢ φ 🡒 φ := impId;
   contradiction;
 
 variable [DecidableEq α]
 
 lemma iff_consistent_insert₁
-  : Tableau.Consistent 𝓢 ((insert φ T), U) ↔ ∀ {Γ Δ : Finset (Formula α)}, (↑Γ ⊆ T) → (↑Δ ⊆ U) → 𝓢 ⊬ φ ⋏ Γ.conj 🡒 Δ.disj := by
+  : (t.insert₁ φ).Consistent 𝓢 ↔ ∀ {Γ Δ : Finset (Formula α)}, (↑Γ ⊆ t.Γ) → (↑Δ ⊆ t.Δ) → 𝓢 ⊬ (insert φ Γ).conj 🡒 Δ.disj := by
   constructor;
   . intro h Γ Δ hΓ hΔ;
     by_contra hC;
     apply h (Γ := insert φ Γ) (Δ := Δ) ?_ hΔ;
-    . exact C!_trans (by simp) hC;
+    . assumption;
     . simp only [Finset.coe_insert];
       apply Set.insert_subset_insert;
       exact hΓ;
   . intro h Γ Δ hΓ hΔ;
     by_contra hC;
-    simp_all only;
     apply h (Γ := Γ.erase φ) (Δ := Δ) (by simpa) hΔ;
-    refine C!_trans ?_ hC;
-    . exact C!_trans CKFConjinsertFConj! $ CFConj_FConj!_of_subset $ Finset.insert_erase_subset φ Γ
+    exact ruleI (CFConjFConj_of_subset (by grind)) hC;
 
-lemma iff_not_consistent_insert₁ : ¬Tableau.Consistent 𝓢 ((insert φ T), U) ↔ ∃ Γ Δ : Finset (Formula α), (↑Γ ⊆ T) ∧ (↑Δ ⊆ U) ∧ 𝓢 ⊢ φ ⋏ Γ.conj 🡒 Δ.disj := by
-  constructor;
-  . contrapose!; apply iff_consistent_insert₁.mpr;
-  . contrapose!; apply iff_consistent_insert₁.mp;
+lemma iff_not_consistent_insert₁ : (t.insert₁ φ).Inconsistent 𝓢  ↔ ∃ Γ Δ : Finset (Formula α), (↑Γ ⊆ t.Γ) ∧ (↑Δ ⊆ t.Δ) ∧ 𝓢 ⊢ (insert φ Γ).conj 🡒 Δ.disj := by
+  apply Iff.trans iff_consistent_insert₁.not
+  grind;
 
-lemma iff_consistent_insert₂ : Tableau.Consistent 𝓢 (T, (insert φ U)) ↔ ∀ {Γ Δ : Finset (Formula α)}, (↑Γ ⊆ T) → (↑Δ ⊆ U) → 𝓢 ⊬ Γ.conj 🡒 φ ⋎ Δ.disj := by
+lemma iff_consistent_insert₂ : (t.insert₂ φ).Consistent 𝓢 ↔ ∀ {Γ Δ : Finset (Formula α)}, (↑Γ ⊆ t.Γ) → (↑Δ ⊆ t.Δ) → 𝓢 ⊬ Γ.conj 🡒 (insert φ Δ).disj := by
   constructor;
   . intro h Γ Δ hΓ hΔ;
     by_contra hC;
     apply h (Γ := Γ) (Δ := insert φ Δ) hΓ ?_;
-    . exact C!_trans hC $ by simp;
+    . assumption;
     . simp only [Finset.coe_insert];
       apply Set.insert_subset_insert;
       exact hΔ;
   . intro h Γ Δ hΓ hΔ;
     by_contra hC;
     apply h (Γ := Γ) (Δ := Δ.erase φ) hΓ (by simpa);
-    exact C!_trans hC $ by
-      refine C!_trans ?_ $ CinsertFDisjAFDisj! (𝓢 := 𝓢) (Γ := Δ.erase φ);
-      apply CDisj₂Disj₂_of_subset;
-      simp only [Finset.mem_toList, Finset.mem_insert, Finset.mem_erase, ne_eq];
-      tauto;
+    apply ruleI hC;
+    apply CFDisjFDisj_of_subset;
+    grind;
 
-lemma iff_not_consistent_insert₂ : ¬Tableau.Consistent 𝓢 (T, (insert φ U)) ↔ ∃ Γ Δ : Finset (Formula α), (↑Γ ⊆ T) ∧ (↑Δ ⊆ U) ∧ 𝓢 ⊢ Γ.conj 🡒 φ ⋎ Δ.disj := by
-  constructor;
-  . contrapose!; apply iff_consistent_insert₂.mpr;
-  . contrapose!; apply iff_consistent_insert₂.mp;
+lemma iff_not_consistent_insert₂ : (t.insert₂ φ).Inconsistent 𝓢  ↔ ∃ Γ Δ : Finset (Formula α), (↑Γ ⊆ t.Γ) ∧ (↑Δ ⊆ t.Δ) ∧ 𝓢 ⊢ Γ.conj 🡒 (insert φ Δ).disj := by
+  apply Iff.trans iff_consistent_insert₂.not;
+  grind;
 
 section Consistent
 
 variable {t : Tableau α}
 
-lemma consistent_either (hCon : t.Consistent 𝓢) (φ : Formula α) : Tableau.Consistent 𝓢 ((insert φ t.1), t.2) ∨ Tableau.Consistent 𝓢 (t.1, (insert φ t.2)) := by
-  by_contra hC;
-  push_neg at hC;
-  have ⟨hC₁, hC₂⟩ := hC;
-
-  obtain ⟨Γ₁, Δ₁, hΓ₁, hΔ₁, h₁⟩ := iff_not_consistent_insert₁.mp hC₁;
-  replace h₁ := left_K!_symm h₁;
-
-  obtain ⟨Γ₂, Δ₂, hΓ₂, hΔ₂, h₂⟩ := iff_not_consistent_insert₂.mp hC₂;
+lemma consistent_either (hCon : t.Consistent 𝓢) (φ : Formula α)
+  : Tableau.Consistent 𝓢 (t.insert₁ φ) ∨ Tableau.Consistent 𝓢 (t.insert₂ φ) := by
+  by_contra! hC;
+  have ⟨h₁, h₂⟩ := hC;
+  obtain ⟨Γ₁, Δ₁, hΓ₁, hΔ₁, h₁⟩ := iff_not_consistent_insert₁.mp h₁;
+  obtain ⟨Γ₂, Δ₂, hΓ₂, hΔ₂, h₂⟩ := iff_not_consistent_insert₂.mp h₂;
   apply @hCon (Γ := Γ₁ ∪ Γ₂) (Δ := Δ₁ ∪ Δ₂) ?_ ?_;
-  . exact C!_trans (C!_trans (by simp) (cut! h₁ h₂)) (by simp);
+  . replace h₁ : 𝓢 ⊢ φ ⋏ Γ₁.conj 🡒 Δ₁.disj := ruleI insert_FConj h₁;
+    replace h₂ : 𝓢 ⊢ Γ₂.conj 🡒 φ ⋎ Δ₂.disj := by
+      apply ruleI;
+      . exact h₂;
+      . sorry;
+    sorry;
   . simp only [Finset.coe_union, Set.union_subset_iff]; tauto;
   . simp only [Finset.coe_union, Set.union_subset_iff]; tauto;
-
-  -- have : 𝓢 ⊢ ⋀(Γ₁ ++ Γ₂) 🡒 ⋁(Δ₁ ++ Δ₂) := C!_trans (K!_left EConj₂AppendKConj₂Conj₂!) $ C!_trans (cut! h₁ h₂) (K!_right EDisj₂AppendADisj₂Disj₂!);
 
 end Consistent
 
 end
 
-abbrev Saturated (t : Tableau α) := ∀ φ : Formula α, φ ∈ t.1 ∨ φ ∈ t.2
+
+@[grind]
+def Saturated (t : Tableau α) := ∀ φ : Formula α, φ ∈ t.Γ ∨ φ ∈ t.Δ
 
 section Saturated
 
-variable [Entailment.Int 𝓢]
+variable [Entailment.VF 𝓢]
 variable {t : Tableau α}
 
-lemma mem₂_of_not_mem₁ (hMat : Saturated t) : φ ∉ t.1 → φ ∈ t.2 := by
-  intro h;
-  cases (hMat φ) with
-  | inl h' => exact absurd h' h;
-  | inr _ => assumption;
+lemma mem₂_of_notMem₁_of_saturated (hMat : Saturated t) : φ ∉ t.Γ → φ ∈ t.Δ := by grind;
+lemma mem₁_of_notMem₂_of_saturated (hMat : Saturated t) : φ ∉ t.Δ → φ ∈ t.Γ := by grind;
 
-lemma mem₁_of_not_mem₂ (hMat : Saturated t) : φ ∉ t.2 → φ ∈ t.1 := by
-  intro h;
-  cases (hMat φ) with
-  | inl _ => assumption;
-  | inr h' => exact absurd h' h;
-
-lemma not_mem₁_iff_mem₂ (hCon : t.Consistent 𝓢) (hMat : Saturated t) : φ ∉ t.1 ↔ φ ∈ t.2 := by
+@[grind .]
+lemma iff_mem₁_notMem₂_of_consistent_saturated (hCon : t.Consistent 𝓢) (hSat : Saturated t) : φ ∈ t.Γ ↔ φ ∉ t.Δ := by
   constructor;
-  . apply mem₂_of_not_mem₁ hMat;
-  . apply Set.disjoint_right.mp $ disjoint_of_consistent hCon;
+  . apply Set.disjoint_right.mp $ Disjoint.symm $ disjoint_of_consistent hCon;
+  . apply mem₁_of_notMem₂_of_saturated hSat;
 
-lemma not_mem₂_iff_mem₁ (hCon : t.Consistent 𝓢) (hMat : Saturated t) : φ ∉ t.2 ↔ φ ∈ t.1 := by
+@[grind .]
+lemma iff_mem₂_notMem₁_of_consistent_saturated (hCon : t.Consistent 𝓢) (hSat : Saturated t) : φ ∈ t.Δ ↔ φ ∉ t.Γ := by
   constructor;
-  . apply mem₁_of_not_mem₂ hMat;
-  . apply Set.disjoint_left.mp $ disjoint_of_consistent hCon;
+  . apply Set.disjoint_left.mp $ Disjoint.symm $ disjoint_of_consistent hCon;
+  . apply mem₂_of_notMem₁_of_saturated hSat;
 
-lemma saturated_duality
-  {t₁ t₂ : Tableau α}
-  (ct₁ : t₁.Consistent 𝓢) (ct₂ : t₂.Consistent 𝓢)
-  (st₁ : Saturated t₁) (st₂ : Saturated t₂)
-  : t₁.1 = t₂.1 ↔ t₁.2 = t₂.2 := by
-  constructor;
-  . intro h;
-    apply Set.eq_of_subset_of_subset;
-    . intro φ hp;
-      apply not_mem₁_iff_mem₂ ct₂ st₂ |>.mp; rw [←h];
-      apply not_mem₁_iff_mem₂ ct₁ st₁ |>.mpr hp;
-    . intro φ hp;
-      apply not_mem₁_iff_mem₂ ct₁ st₁ |>.mp; rw [h];
-      apply not_mem₁_iff_mem₂ ct₂ st₂ |>.mpr hp;
-  . intro h;
-    apply Set.eq_of_subset_of_subset;
-    . intro φ hp;
-      apply not_mem₂_iff_mem₁ ct₂ st₂ |>.mp; rw [←h];
-      apply not_mem₂_iff_mem₁ ct₁ st₁ |>.mpr hp;
-    . intro φ hp;
-      apply not_mem₂_iff_mem₁ ct₁ st₁ |>.mp; rw [h];
-      apply not_mem₂_iff_mem₁ ct₂ st₂ |>.mpr hp;
+lemma saturated_duality {t₁ t₂ : Tableau α} (ct₁ : t₁.Consistent 𝓢) (ct₂ : t₂.Consistent 𝓢) (st₁ : Saturated t₁) (st₂ : Saturated t₂) :
+  t₁.Γ = t₂.Γ ↔ t₁.Δ = t₂.Δ := by grind;
 
 end Saturated
 
-lemma emptyset_consistent [Entailment.Int 𝓢] [DecidableEq α] [H_consis : Entailment.Consistent 𝓢] : Consistent 𝓢 ⟨∅, ∅⟩ := by
+lemma emptyset_consistent [Entailment.VF 𝓢] [DecidableEq α] [H_consis : Entailment.Consistent 𝓢] : Consistent 𝓢 ⟨∅, ∅⟩ := by
   intro Γ Δ hΓ hΔ;
   by_contra hC;
   obtain ⟨ψ, hψ⟩ := H_consis.exists_unprovable;
@@ -187,7 +164,7 @@ lemma emptyset_consistent [Entailment.Int 𝓢] [DecidableEq α] [H_consis : Ent
   simp only [Set.subset_empty_iff, Finset.coe_eq_empty] at hΓ hΔ;
   subst hΓ hΔ;
   simp only [Finset.conj_empty, Finset.disj_empty] at hC;
-  exact of_O! (hC ⨀ C!_id);
+  exact Corsi.of_O (hC ⨀ (by simp));
 
 section lindenbaum
 
@@ -197,7 +174,7 @@ variable {t : Tableau α}
 open Classical
 open Encodable
 
-noncomputable def lindenbaum_next (φ : Formula α) (t : Tableau α) : Tableau α := if Tableau.Consistent 𝓢 (insert φ t.1, t.2) then (insert φ t.1, t.2) else (t.1, insert φ t.2)
+noncomputable def lindenbaum_next (φ : Formula α) (t : Tableau α) : Tableau α := if Tableau.Consistent 𝓢 (t.insert₁ φ) then (t.insert₁ φ) else (t.insert₂ φ)
 
 noncomputable def lindenbaum_next_indexed [Encodable α] (t : Tableau α) : ℕ → Tableau α
   | 0 => t
@@ -207,14 +184,14 @@ noncomputable def lindenbaum_next_indexed [Encodable α] (t : Tableau α) : ℕ 
     | none => lindenbaum_next_indexed t i
 local notation:max t"[" i "]" => lindenbaum_next_indexed 𝓢 t i
 
-def lindenbaum_maximal [Encodable α] (t : Tableau α) : Tableau α := (⋃ i, t[i].1, ⋃ i, t[i].2)
+def lindenbaum_maximal [Encodable α] (t : Tableau α) : Tableau α := ⟨⋃ i, t[i].1, ⋃ i, t[i].2⟩
 local notation:max t"∞" => lindenbaum_maximal 𝓢 t
 
 @[simp] lemma lindenbaum_next_indexed_zero [Encodable α] {t : Tableau α} : (t.lindenbaum_next_indexed 𝓢 0) = t := by simp [lindenbaum_next_indexed]
 
 variable {𝓢}
 
-lemma next_parametericConsistent [Entailment.Int 𝓢] (consistent : t.Consistent 𝓢) (φ : Formula α) : (t.lindenbaum_next 𝓢 φ).Consistent 𝓢 := by
+lemma next_parametericConsistent [Entailment.VF 𝓢] (consistent : t.Consistent 𝓢) (φ : Formula α) : (t.lindenbaum_next 𝓢 φ).Consistent 𝓢 := by
   dsimp [lindenbaum_next];
   split;
   . simpa;
@@ -224,7 +201,7 @@ lemma next_parametericConsistent [Entailment.Int 𝓢] (consistent : t.Consisten
 
 variable [Encodable α]
 
-lemma lindenbaum_next_indexed_parametricConsistent_succ [Entailment.Int 𝓢] {i : ℕ} : Consistent 𝓢 t[i] → Consistent 𝓢 t[i + 1] := by
+lemma lindenbaum_next_indexed_parametricConsistent_succ [Entailment.VF 𝓢] {i : ℕ} : Consistent 𝓢 t[i] → Consistent 𝓢 t[i + 1] := by
   dsimp [lindenbaum_next_indexed];
   split;
   . intro h;
@@ -238,7 +215,7 @@ lemma mem_lindenbaum_next_indexed (t) (φ : Formula α) : φ ∈ t[(encode φ) +
   . left; tauto;
   . right; tauto;
 
-lemma lindenbaum_next_indexed_parametricConsistent [Entailment.Int 𝓢] (consistent : t.Consistent 𝓢) (i : ℕ) : t[i].Consistent 𝓢 := by
+lemma lindenbaum_next_indexed_parametricConsistent [Entailment.VF 𝓢] (consistent : t.Consistent 𝓢) (i : ℕ) : t[i].Consistent 𝓢 := by
   induction i with
   | zero => simpa;
   | succ i ih => apply lindenbaum_next_indexed_parametricConsistent_succ; assumption;
@@ -309,7 +286,7 @@ lemma exists_finset_lindenbaum_index₂ {Δ : Finset _} (hΓ : ↑Δ ⊆ ⋃ i, 
   apply hΔ;
   simpa;
 
-lemma exists_parametricConsistent_saturated_tableau [Entailment.Int 𝓢] (hCon : t.Consistent 𝓢) : ∃ u, t ⊆ u ∧ (Tableau.Consistent 𝓢 u) ∧ (Saturated u) := by
+lemma exists_parametricConsistent_saturated_tableau [Entailment.VF 𝓢] (hCon : t.Consistent 𝓢) : ∃ u, t ⊆ u ∧ (Tableau.Consistent 𝓢 u) ∧ (Saturated u) := by
   use t∞;
   refine ⟨?subset, ?consistent, ?saturated⟩;
   case subset => constructor <;> apply Set.subset_iUnion_of_subset 0 (by simp);
@@ -338,45 +315,42 @@ end Tableau
 
 open Tableau
 
-def SaturatedConsistentTableau (𝓢 : S) := {t : Tableau α // Saturated t ∧ t.Consistent 𝓢}
+@[ext]
+structure SaturatedConsistentTableau (𝓢 : S) extends Tableau α where
+  saturated : Saturated toTableau
+  consistent : Consistent 𝓢 toTableau
 
 namespace SaturatedConsistentTableau
 
-lemma consistent (t : SaturatedConsistentTableau 𝓢) : Consistent 𝓢 t.1 := t.2.2
-
-lemma saturated (t : SaturatedConsistentTableau 𝓢) : Saturated t.1 := t.2.1
-
 variable {t₀ : Tableau α} {φ ψ : Formula α}
 
-lemma lindenbaum [Entailment.Int 𝓢] [Encodable α] (hCon : t₀.Consistent 𝓢) : ∃ (t : SaturatedConsistentTableau 𝓢), t₀ ⊆ t.1 := by
+attribute [simp, grind .] saturated consistent
+
+lemma lindenbaum [Entailment.VF 𝓢] [Encodable α] (hCon : t₀.Consistent 𝓢) : ∃ (t : SaturatedConsistentTableau 𝓢), t₀ ⊆ t.toTableau := by
   obtain ⟨t, ht, hCon, hMax⟩ := Tableau.lindenbaum hCon;
   exact ⟨⟨t, hMax, hCon⟩, ht⟩;
 
-instance [Entailment.Consistent 𝓢] [Entailment.Int 𝓢] [DecidableEq α] [Encodable α] : Nonempty (SaturatedConsistentTableau 𝓢) := ⟨lindenbaum Tableau.emptyset_consistent |>.choose⟩
+instance [Entailment.Consistent 𝓢] [Entailment.VF 𝓢] [DecidableEq α] [Encodable α] : Nonempty (SaturatedConsistentTableau 𝓢) := ⟨lindenbaum Tableau.emptyset_consistent |>.choose⟩
 
 variable {t t₁ t₂ : SaturatedConsistentTableau 𝓢}
 
-lemma not_mem₂ {Γ : Finset (Formula α)} (hΓ : ↑Γ ⊆ t.1.1) (h : 𝓢 ⊢ Γ.conj 🡒 ψ) : ψ ∉ t.1.2 := t.1.not_mem₂ t.consistent hΓ h
+lemma not_mem₂ {Γ : Finset (Formula α)} (hΓ : ↑Γ ⊆ t.Γ) (h : 𝓢 ⊢ Γ.conj 🡒 ψ) : ψ ∉ t.Δ := t.toTableau.not_mem₂ t.consistent hΓ h
 
-variable [Entailment.Int 𝓢]
+variable [Entailment.VF 𝓢]
 
-@[simp] lemma disjoint : Disjoint t.1.1 t.1.2 := t.1.disjoint_of_consistent t.2.2
+@[simp, grind .] lemma disjoint : Disjoint t.Γ t.Δ := t.toTableau.disjoint_of_consistent t.consistent
 
-lemma iff_not_mem₁_mem₂ : φ ∉ t.1.1 ↔ φ ∈ t.1.2 := Tableau.not_mem₁_iff_mem₂ t.consistent t.saturated
+lemma iff_mem₁_notMem₂ : φ ∈ t.Γ ↔ φ ∉ t.Δ := t.toTableau.iff_mem₁_notMem₂_of_consistent_saturated t.consistent t.saturated
+lemma iff_mem₂_notMem₁ : φ ∈ t.Δ ↔ φ ∉ t.Γ := t.toTableau.iff_mem₂_notMem₁_of_consistent_saturated t.consistent t.saturated
 
-lemma iff_not_mem₂_mem₁ : φ ∉ t.1.2 ↔ φ ∈ t.1.1 := Tableau.not_mem₂_iff_mem₁ t.consistent t.saturated
+attribute [grind =_] iff_mem₁_notMem₂ iff_mem₂_notMem₁
 
-lemma saturated_duality: t₁.1.1 = t₂.1.1 ↔ t₁.1.2 = t₂.1.2 := Tableau.saturated_duality t₁.consistent t₂.consistent t₁.saturated t₂.saturated
+@[grind =] lemma saturated_duality: t₁.Γ = t₂.Γ ↔ t₁.Δ = t₂.Δ := Tableau.saturated_duality t₁.consistent t₂.consistent t₁.saturated t₂.saturated
 
-lemma equality_of₁ (e₁ : t₁.1.1 = t₂.1.1) : t₁ = t₂ := by
-  have e := Tableau.equality_def.mpr ⟨e₁, (saturated_duality.mp e₁)⟩;
-  calc
-    t₁ = ⟨t₁.1, t₁.saturated, t₁.consistent⟩ := by rfl;
-    _  = ⟨t₂.1, t₂.saturated, t₂.consistent⟩ := by simp [e];
-    _  = t₂                                  := by rfl;
+@[grind <=] lemma equality_of₁ (e₁ : t₁.Γ = t₂.Γ) : t₁ = t₂ := by ext <;> grind;
+@[grind <=] lemma equality_of₂ (e₂ : t₁.Δ = t₂.Δ) : t₁ = t₂ := by ext <;> grind;
 
-lemma equality_of₂ (e₂ : t₁.1.2 = t₂.1.2) : t₁ = t₂ := equality_of₁ $ saturated_duality.mpr e₂
-
+/-
 section
 
 variable [DecidableEq α] [Encodable α]
@@ -424,60 +398,66 @@ lemma iff_provable_mem₁ : 𝓢 ⊢ φ ↔ ∀ t : SaturatedConsistentTableau �
     exact Context.emptyPrf! $ iff_provable_include₁.mpr $ by tauto;
 
 end
+-/
 
 section Saturated
 
-lemma mdp_mem₁_provable (h : 𝓢 ⊢ φ 🡒 ψ) (hp₁ : φ ∈ t.1.1) : ψ ∈ t.1.1 := by
-  apply iff_not_mem₂_mem₁.mp;
+lemma imp_closed₁ (h : 𝓢 ⊢ φ 🡒 ψ) (hp₁ : φ ∈ t.1.1) : ψ ∈ t.1.1 := by
   by_contra hq₂;
-  apply by simpa using t.consistent (Γ := {φ}) (Δ := {ψ}) (by simpa) (by simpa);
-  exact h;
+  apply t.consistent (Γ := {φ}) (Δ := {ψ});
+  . grind;
+  . grind;
+  . simpa;
 
-lemma mdp_mem₂_provable (h : 𝓢 ⊢ φ 🡒 ψ) (hp₁ : ψ ∈ t.1.2) : φ ∈ t.1.2 := by
-  by_contra hq₂;
-  have := iff_not_mem₂_mem₁.mpr $ mdp_mem₁_provable h $ iff_not_mem₂_mem₁.mp hq₂;
-  contradiction;
+lemma imp_closed₂ (h : 𝓢 ⊢ φ 🡒 ψ) (hp₂ : ψ ∈ t.1.2) : φ ∈ t.1.2 := by
+  contrapose! hp₂;
+  grind [imp_closed₁ h];
 
-@[simp] lemma mem₁_verum : ⊤ ∈ t.1.1 := by
-  apply iff_not_mem₂_mem₁.mp;
+@[simp, grind .]
+lemma mem₁_verum : ⊤ ∈ t.Γ := by
   by_contra hC;
-  apply by simpa using t.consistent (Γ := ∅) (Δ := {⊤}) (by simp) (by simpa);
-  simp;
+  apply t.consistent (Γ := ∅) (Δ := {⊤});
+  . grind;
+  . grind;
+  . simp;
 
-@[simp] lemma not_mem₁_falsum : ⊥ ∉ t.1.1 := by
+@[simp, grind .]
+lemma notMem₁_falsum : ⊥ ∉ t.Γ := by
   by_contra hC;
-  have : 𝓢 ⊬ ⊥ 🡒 ⊥ := by simpa using t.consistent (Γ := {⊥}) (Δ := ∅) (by simpa) (by simp);
-  apply this;
-  simp;
+  apply t.consistent (Γ := {⊥}) (Δ := ∅);
+  . grind;
+  . grind;
+  . simp;
 
-@[simp] lemma mem₂_falsum : ⊥ ∈ t.1.2 := iff_not_mem₁_mem₂.mp not_mem₁_falsum
+@[simp, grind .]
+lemma mem₂_falsum : ⊥ ∈ t.Δ := by grind;
 
-lemma mem₁_of_provable : 𝓢 ⊢ φ → φ ∈ t.1.1 := by
+lemma mem₁_of_provable (t : SaturatedConsistentTableau 𝓢) : 𝓢 ⊢ φ → φ ∈ t.Γ := by
   intro h;
-  exact mdp_mem₁_provable (C!_of_conseq! h) mem₁_verum;
+  apply imp_closed₁ (φ := ⊤);
+  . apply Corsi.af h;
+  . grind;
 
-lemma mdp_mem₁ [DecidableEq α] (h : φ 🡒 ψ ∈ t.1.1) (hp : φ ∈ t.1.1) : ψ ∈ t.1.1 := by
-  apply iff_not_mem₂_mem₁.mp;
-  by_contra hC;
-  apply t.consistent (Γ := {φ, φ 🡒 ψ}) (Δ := {ψ}) ?_ (by simpa);
-  . apply CFConj_CDisj!_of_innerMDP (φ := φ) (ψ := ψ) <;> simp;
-  . simp only [Finset.coe_insert, Finset.coe_singleton];
-    apply Set.doubleton_subset.mpr;
-    tauto;
+open Entailment.Corsi
 
-lemma iff_mem₁_and [DecidableEq α] : φ ⋏ ψ ∈ t.1.1 ↔ φ ∈ t.1.1 ∧ ψ ∈ t.1.1 := by
+@[grind =>]
+lemma iff_mem₁_and [DecidableEq α] : φ ⋏ ψ ∈ t.Γ ↔ φ ∈ t.Γ ∧ ψ ∈ t.Γ := by
   constructor;
-  . intro h; constructor <;> exact mdp_mem₁_provable (by simp) h
+  . intro h; constructor <;> exact imp_closed₁ (by simp) h
   . rintro ⟨hp, hq⟩;
-    apply iff_not_mem₂_mem₁.mp;
     by_contra hC;
-    apply t.consistent (Γ := {φ, ψ}) (Δ := {φ ⋏ ψ}) ?_ (by simp_all);
-    . apply CFConj_CDisj!_of_K_intro (φ := φ) (ψ := ψ) <;> simp;
-    . simp only [Finset.coe_insert, Finset.coe_singleton];
-      apply Set.doubleton_subset.mpr;
-      tauto;
+    apply t.consistent (Γ := {φ, ψ}) (Δ := {φ ⋏ ψ});
+    . grind;
+    . grind;
+    . rw [Finset.disj_singleton];
+      apply ruleC <;> exact mem_fconj (by simp);
 
-lemma iff_mem₁_conj₂ [DecidableEq α] {Γ : List (Formula α)} : ⋀Γ ∈ t.1.1 ↔ ∀ φ ∈ Γ, φ ∈ t.1.1 := by
+@[grind =>]
+lemma iff_mem₂_and [DecidableEq α] : φ ⋏ ψ ∈ t.Δ ↔ φ ∈ t.Δ ∨ ψ ∈ t.Δ := by grind;
+
+attribute [grind =] List.conj₂_nil List.conj₂_singleton List.conj₂_cons_nonempty
+
+lemma iff_mem₁_conj₂ [DecidableEq α] {Γ : List (Formula α)} : ⋀Γ ∈ t.Γ ↔ ∀ φ ∈ Γ, φ ∈ t.Γ := by
   induction Γ using List.induction_with_singleton with
   | hcons φ Γ Γ_nil ih =>
     simp only [(List.conj₂_cons_nonempty Γ_nil), List.mem_cons];
@@ -487,59 +467,26 @@ lemma iff_mem₁_conj₂ [DecidableEq α] {Γ : List (Formula α)} : ⋀Γ ∈ t
       . exact ih.mp (iff_mem₁_and.mp h |>.2) _ hp;
     . intro h;
       apply iff_mem₁_and.mpr;
-      simp_all;
+      grind;
   | _ => simp;
 
-lemma iff_mem₁_fconj [DecidableEq α] {Γ : Finset (Formula α)} : Γ.conj ∈ t.1.1 ↔ ↑Γ ⊆ t.1.1 := by
+lemma iff_mem₁_fconj [DecidableEq α] {Γ : Finset (Formula α)} : Γ.conj ∈ t.Γ ↔ ↑Γ ⊆ t.Γ := by
+  apply Iff.trans iff_mem₁_conj₂;
+  grind [Finset.mem_toList];
+
+@[grind =>]
+lemma iff_mem₁_or [DecidableEq α] : φ ⋎ ψ ∈ t.Γ ↔ φ ∈ t.Γ ∨ ψ ∈ t.Γ := by
   constructor;
-  . intro h φ hφ;
-    apply iff_mem₁_conj₂ (Γ := Γ.toList) (t := t) |>.mp;
-    . apply mdp_mem₁_provable ?_ h; simp;
-    . simpa;
   . intro h;
-    apply mdp_mem₁_provable ?_ $ iff_mem₁_conj₂ (Γ := Γ.toList) (t := t) |>.mpr $ by
-      intro φ hφ;
-      apply h;
-      simp_all;
-    simp;
+    by_contra! hC;
+    apply t.consistent (Γ := {φ ⋎ ψ}) (Δ := {φ, ψ}) (by simp_all);
+    . grind;
+    . rw [Finset.conj_singleton];
+      apply ruleD <;> apply mem_fdisj (by simp);
+  . rintro (h | h) <;> apply imp_closed₁ (by simp) h;
 
-private lemma of_mem₁_or [DecidableEq α] : φ ⋎ ψ ∈ t.1.1 → (φ ∈ t.1.1 ∨ ψ ∈ t.1.1) := by
-  intro h;
-  by_contra hC; push_neg at hC;
-  apply t.consistent (Γ := {φ ⋎ ψ}) (Δ := {φ, ψ}) (by simp_all) ?_;
-  . apply CFConj_CDisj!_of_A (φ := φ) (ψ := ψ) <;> simp;
-  . simp only [Finset.coe_insert, Finset.coe_singleton];
-    apply Set.doubleton_subset.mpr;
-    constructor;
-    . exact iff_not_mem₁_mem₂.mp hC.1;
-    . exact iff_not_mem₁_mem₂.mp hC.2;
-
-private lemma of_mem₂_or : φ ⋎ ψ ∈ t.1.2 → φ ∈ t.1.2 ∧ ψ ∈ t.1.2 := by
-  contrapose;
-  suffices (φ ∉ t.1.2 ∨ ψ ∉ t.1.2) → φ ⋎ ψ ∉ t.1.2 by tauto;
-  rintro (hφ | hψ);
-  . apply iff_not_mem₂_mem₁.mpr;
-    exact mdp_mem₁_provable or₁! $ iff_not_mem₂_mem₁.mp hφ;
-  . apply iff_not_mem₂_mem₁.mpr;
-    exact mdp_mem₁_provable or₂! $ iff_not_mem₂_mem₁.mp hψ;
-
-lemma iff_mem₁_or [DecidableEq α] : φ ⋎ ψ ∈ t.1.1 ↔ φ ∈ t.1.1 ∨ ψ ∈ t.1.1 := by
-  constructor;
-  . apply of_mem₁_or;
-  . intro h;
-    cases h with
-    | inl h => exact mdp_mem₁_provable or₁! h;
-    | inr h => exact mdp_mem₁_provable or₂! h;
-
-lemma iff_mem₂_or [DecidableEq α] : φ ⋎ ψ ∈ t.1.2 ↔ φ ∈ t.1.2 ∧ ψ ∈ t.1.2 := by
-  constructor;
-  . apply of_mem₂_or;
-  . contrapose;
-    push_neg;
-    intro hφψ hφ;
-    rcases iff_mem₁_or.mp $ iff_not_mem₂_mem₁.mp hφψ with (hφ | hψ);
-    . have := iff_not_mem₂_mem₁.mpr hφ; contradiction;
-    . exact iff_not_mem₂_mem₁.mpr hψ;
+@[grind =>]
+lemma iff_mem₂_or [DecidableEq α] : φ ⋎ ψ ∈ t.Δ ↔ φ ∈ t.Δ ∧ ψ ∈ t.Δ := by grind;
 
 lemma iff_mem₂_disj [DecidableEq α] {Γ : List (Formula α)} : ⋁Γ ∈ t.1.2 ↔ ∀ φ ∈ Γ, φ ∈ t.1.2 := by
   induction Γ using List.induction_with_singleton with
@@ -555,87 +502,41 @@ lemma iff_mem₂_disj [DecidableEq α] {Γ : List (Formula α)} : ⋁Γ ∈ t.1.
   | _ => simp;
 
 lemma iff_mem₂_fdisj [DecidableEq α] {Γ : Finset (Formula α)} : Γ.disj ∈ t.1.2 ↔ ↑Γ ⊆ t.1.2 := by
-  apply Iff.trans $ show Γ.disj ∈ t.1.2 ↔ ⋁Γ.toList ∈ t.1.2 by constructor <;> apply mdp_mem₂_provable $ by simp;
   apply Iff.trans iff_mem₂_disj;
-  simp_all only [Finset.mem_toList];
-  rfl;
+  grind [Finset.mem_toList]
 
-lemma of_mem₁_imp [DecidableEq α] : φ 🡒 ψ ∈ t.1.1 → (φ ∈ t.1.2 ∨ ψ ∈ t.1.1) := by
-  intro h;
+@[grind =>]
+lemma of_mem₁_imp [DecidableEq α] [HasAxiomRfl 𝓢] (h : φ 🡒 ψ ∈ t.Γ) (hp : φ ∈ t.Γ) : ψ ∈ t.Γ := by
   by_contra hC;
-  push_neg at hC;
-  exact hC.2 $ mdp_mem₁ h $ iff_not_mem₂_mem₁.mp hC.1
+  apply t.consistent (Γ := {φ, φ 🡒 ψ}) (Δ := {ψ});
+  . grind;
+  . grind;
+  . rw [Finset.disj_singleton];
+    apply ruleI (ψ := φ ⋏ (φ 🡒 ψ));
+    . apply ruleC <;> exact mem_fconj (by simp);
+    . simp;
 
-lemma of_mem₁_imp' [DecidableEq α] : φ 🡒 ψ ∈ t.1.1 → (φ ∈ t.1.1 → ψ ∈ t.1.1) := by
-  intro h h₁;
-  apply or_iff_not_imp_left.mp $ of_mem₁_imp h;
-  apply iff_not_mem₂_mem₁.mpr h₁;
+lemma of_mem₁_imp' [DecidableEq α] [HasAxiomRfl 𝓢] : φ 🡒 ψ ∈ t.1.1 → (φ ∈ t.1.2 ∨ ψ ∈ t.1.1) := by grind [of_mem₁_imp];
 
-lemma of_mem₁_neg [DecidableEq α] (h : ∼φ ∈ t.1.1) : φ ∈ t.1.2 := by
-  rcases of_mem₁_imp h with (hC | hC);
-  . assumption;
-  . exfalso;
-    exact SaturatedConsistentTableau.not_mem₁_falsum hC;
 
-lemma of_mem₁_neg' [DecidableEq α] (h : ∼φ ∈ t.1.1) : φ ∉ t.1.1 := by
-  apply iff_not_mem₁_mem₂.mpr;
-  apply of_mem₁_neg h;
+@[grind =>]
+lemma of_mem₁_neg [DecidableEq α] [HasAxiomRfl 𝓢] (h : ∼φ ∈ t.1.1) : φ ∉ t.1.1 := by grind [of_mem₁_imp];
 
-private lemma of_mem₂_imp [DecidableEq α] [Encodable α] [Entailment.Cl 𝓢] : φ 🡒 ψ ∈ t.1.2 → (φ ∈ t.1.1 ∧ ψ ∈ t.1.2) := by
+lemma of_mem₁_neg' [DecidableEq α] [HasAxiomRfl 𝓢] (h : ∼φ ∈ t.1.1) : φ ∈ t.1.2 := by grind;
+
+
+private lemma of_mem₂_imp [DecidableEq α] [Encodable α] [HasAxiomRfl 𝓢] [Entailment.Cl 𝓢] : φ 🡒 ψ ∈ t.1.2 → (φ ∈ t.1.1 ∧ ψ ∈ t.1.2) := by
   intro h;
-  by_contra hC;
-  replace hC := not_and_or.mp hC;
+  set_option push_neg.use_distrib true in by_contra! hC;
   rcases hC with (hφ | hψ);
-  . have : φ ⋎ (φ 🡒 ψ) ∈ t.1.1 := iff_provable_mem₁.mp (A!_replace_right lem! CNC!) t;
-    rcases iff_mem₁_or.mp this with (_ | _);
-    . contradiction;
-    . have := iff_not_mem₁_mem₂.mpr h;
-      contradiction;
-  . have : ψ 🡒 (φ 🡒 ψ) ∈ t.1.1 := iff_provable_mem₁.mp implyK! t;
-    have : φ 🡒 ψ ∉ t.1.2 := iff_not_mem₂_mem₁.mpr $ mdp_mem₁ this (iff_not_mem₂_mem₁.mp hψ);
-    contradiction;
+  . rcases iff_mem₁_or.mp (mem₁_of_provable t (show 𝓢 ⊢ φ ⋎ (φ 🡒 ψ) by sorry)) with (_ | _) <;> grind;
+  . exact (iff_mem₁_notMem₂.mp $ of_mem₁_imp (mem₁_of_provable t (by sorry)) $ iff_mem₁_notMem₂.mpr hψ) h;
 
-lemma iff_mem₁_imp [DecidableEq α] [Encodable α] [Entailment.Cl 𝓢] : φ 🡒 ψ ∈ t.1.1 ↔ (φ ∈ t.1.2 ∨ ψ ∈ t.1.1) := by
-  constructor;
-  . apply of_mem₁_imp;
-  . contrapose;
-    push_neg;
-    intro hφψ;
-    rcases of_mem₂_imp $ iff_not_mem₁_mem₂.mp hφψ with ⟨hφ, hψ⟩;
-    constructor;
-    . exact iff_not_mem₂_mem₁.mpr hφ;
-    . exact iff_not_mem₁_mem₂.mpr hψ;
+lemma iff_mem₁_imp [DecidableEq α] [Encodable α] [HasAxiomRfl 𝓢] [Entailment.Cl 𝓢] : φ 🡒 ψ ∈ t.1.1 ↔ (φ ∈ t.1.2 ∨ ψ ∈ t.1.1) := by
+  grind only [of_mem₁_imp, of_mem₂_imp, iff_mem₂_notMem₁, iff_mem₁_notMem₂];
 
-lemma iff_mem₂_imp [DecidableEq α] [Encodable α] [Entailment.Cl 𝓢] : φ 🡒 ψ ∈ t.1.2 ↔ (φ ∈ t.1.1 ∧ ψ ∈ t.1.2) := by
-  constructor;
-  . apply of_mem₂_imp;
-  . contrapose;
-    push_neg;
-    intro hφψ hφ;
-    rcases of_mem₁_imp $ iff_not_mem₂_mem₁.mp hφψ with (hφ | hψ);
-    . have := iff_not_mem₁_mem₂.mpr hφ; contradiction;
-    . exact iff_not_mem₂_mem₁.mpr hψ;
-
-lemma not_mem₁_neg_of_mem₁ [DecidableEq α] : φ ∈ t.1.1 → ∼φ ∉ t.1.1 := by
-  intro hp;
-  by_contra hnp;
-  have := iff_mem₁_and.mpr ⟨hp, hnp⟩;
-  have : ⊥ ∈ t.1.1 := mdp_mem₁_provable CKNO! this;
-  have : ⊥ ∉ t.1.1 := not_mem₁_falsum
-  contradiction;
-
-lemma mem₂_neg_of_mem₁ [DecidableEq α] : φ ∈ t.1.1 → ∼φ ∈ t.1.2 := by
-  intro h;
-  exact iff_not_mem₁_mem₂ (φ := ∼φ) (t := t) |>.mp $ not_mem₁_neg_of_mem₁ h;
-
-lemma mdp₁_mem [DecidableEq α] (hp : φ ∈ t.1.1) (h : φ 🡒 ψ ∈ t.1.1) : ψ ∈ t.1.1 := by
-  apply iff_not_mem₂_mem₁.mp;
-  by_contra hC;
-  apply t.consistent (Γ := {φ, φ 🡒 ψ}) (Δ := {ψ}) ?_ (by simpa);
-  . apply CFConj_CDisj!_of_innerMDP (φ := φ) (ψ := ψ) <;> simp;
-  . simp only [Finset.coe_insert, Finset.coe_singleton];
-    apply Set.doubleton_subset.mpr;
-    constructor <;> assumption;
+lemma iff_mem₂_imp [DecidableEq α] [Encodable α] [HasAxiomRfl 𝓢] [Entailment.Cl 𝓢] : φ 🡒 ψ ∈ t.1.2 ↔ (φ ∈ t.1.1 ∧ ψ ∈ t.1.2) := by
+  grind only [of_mem₁_imp, of_mem₂_imp, iff_mem₂_notMem₁, iff_mem₁_notMem₂];
 
 end Saturated
 
